% vim: nu expandtab shiftwidth=2 softtabstop=2 foldmethod=marker

\section{Exam Guide 2}
\begin{enumerate}
\item [] Find the general solution in closed form to each recurrence relation. For full credits, you need to justify your answers (if you apply some theorem, you need to cite them).
\item $A_{n}=A_{n-1}-3^{n}+7n$
  \begin{itemize}
  \item First, we solve the homogeneous part, $A_{n}=A_{n-1}$
    \begin{itemize}
    \item The solution is $A_{n}=A_{0}$
    \end{itemize}
  \item Now, split it into simpler heterogeneous equations, and then combine them later. $A_{n}=A_{n-1}-3^{n}$ and $A_{n}=A_{n-1}+7n$
  \item $A_{n}=A_{n-1}-3^{n}$
    \begin{itemize}
    \item The formula is $$F_{n}=c^{n}F_{0} + \sum\limits_{i=0}^{n-1}c^{i}f(n-i)$$
    \item In this problem, $c=1$ and $f(n)=-3^{n}$
    \item Due to $f(n)=-3^{n}$ being an exponential equation, defined by ($f(n)=b^{n}$ where $n\neq0$), we modify the formula. In this case, $b=-3$, as $c\neq b$, we modify the formula to be $$F_{n}=c^{n}F_{0} + b^{n}\left(\frac{(\frac{c}{b})^{n}-1}{(\frac{c}{b})-1}\right)$$
    \item Plugging everything into the formula, we get $$A_{n}=1^{n}A_{0} - 3^{n}\left(\frac{(\frac{1}{-3})^{n}-1}{(\frac{1}{-3})-1}\right)$$
    \end{itemize}
  \item $A_{n}=A_{n-1}+7n$
    \begin{itemize}
    \item The formula is $$F_{n}=c^{n}F_{0} + \sum\limits_{i=0}^{n-1}c^{i}f(n-i)$$
    \item In this problem, $c=1$ and $f(n)=7n$
    \item Plugging everything into the formula, we get $$F_{n}=1^{n}F_{0} + \sum\limits_{i=0}^{n-1}1^{i}7(n-i)$$
    \item $$F_{n}=F_{0} + \sum\limits_{i=0}^{n-1}7(n-i)$$
    \item $$F_{n}=F_{0} + 7\sum\limits_{i=0}^{n-1}(n-i)$$
    \item $F_{n}=F_{0} + 7\left(\frac{n^{2}+n}{2}\right)$
    \item $F_{n}=F_{0} + 7\left(\frac{n\left(n+1\right)}{2}\right)$
    \item $F_{n}=F_{0} + \left(\frac{7n\left(n+1\right)}{2}\right)$
    \end{itemize}
  \item Now we put it all together and get the solution.
  \item $A_{n}=A_{0}-3^{n}\left(\frac{(\frac{1}{-3})^{n}-1}{(\frac{1}{-3}-1}\right)+\left(\frac{7n\left(n+1\right)}{2}\right)$
  \end{itemize} 
\item $F(n)=b*F\left(\left\lfloor\frac{n}{2}\right\rfloor\right)+cn+a$
  \begin{itemize}
  \item Use substitution $a=d$, $b=e$, $c=f$ in order to avoide conflicts with common variables in formulas
  \item $F(n)=e*F\left(\left\lfloor\frac{n}{2}\right\rfloor\right)+fn+d$
  \item $F\left(\left\lfloor\frac{n}{2}\right\rfloor\right)=e*F\left(\left\lfloor\frac{\left\lfloor\frac{n}{2}\right\rfloor}{2}\right\rfloor\right)+f\left\lfloor\frac{n}{2}\right\rfloor+d$ after the first substitution
  \item $F\left(\left\lfloor\frac{n}{2}\right\rfloor\right)=e*F\left(\left\lfloor\frac{n}{2^{2}}\right\rfloor\right)+f\left\lfloor\frac{n}{2}\right\rfloor+d$
  \item Then $F\left(\left\lfloor\frac{n}{2}\right\rfloor\right)=e^{2}*F\left(\left\lfloor\frac{n}{2^{2}}\right\rfloor\right)+ef\left\lfloor\frac{n}{2}\right\rfloor+fn+ed+d$
  \item $F\left(\left\lfloor\frac{n}{2^{2}}\right\rfloor\right)=e^{2}*F\left(\left\lfloor\frac{\left\lfloor\frac{n}{2^{2}}\right\rfloor}{2}\right\rfloor\right)+ef\left\lfloor\frac{n}{2^{2}}\right\rfloor+d$ after the second substitution
  \item $F\left(\left\lfloor\frac{n}{2^{2}}\right\rfloor\right)=e^{2}*F\left(\left\lfloor\frac{n}{2^{3}}\right\rfloor\right)+ef\left\lfloor\frac{n}{2^{2}}\right\rfloor+d$
  \item Then $F\left(\left\lfloor\frac{n}{2^{2}}\right\rfloor\right)=e^{3}*F\left(\left\lfloor\frac{n}{2^{3}}\right\rfloor\right)+e^{2}f\left\lfloor\frac{n}{2^{2}}\right\rfloor++ef\left\lfloor\frac{n}{2}\right\rfloor+fn+e^{2}d+ed+d$
  \item $F(n)=e^{k}*F\left(\left\lfloor\frac{\left\lfloor\frac{n}{2^{k}}\right\rfloor}{2}\right\rfloor\right)+\sum\limits_{i=0}^{k-1}e^{i}f\left\lfloor\frac{n}{2^{i}}\right\rfloor+\sum\limits_{i=0}^{k-1}e^{i}d$ after the k-1 substitution
  \item Now to get the exact solution. $k=\left\lfloor\log{n}\right\rfloor$, and $F\left(\left\lfloor\frac{n}{2^{k}}\right\rfloor\right)=a$ for some constant a.
  \item $F(n)=e^{\lfloor\log{n}\rfloor}a+\sum\limits_{i=0}^{\lfloor\log{n}\rfloor-1}e^{i}f\left\lfloor\frac{n}{2^{i}}\right\rfloor+\sum\limits_{i=0}^{\lfloor\log{n}\rfloor-1}e^{i}d$
  \end{itemize}
\item $F(n)=G(n+1)$ $F(n)=bF\left(\left\lfloor\frac{n-1}{2}\right\rfloor\right)+f(n)$ where $n>0$
\end{enumerate}
